\documentclass[./\jobname.tex]{subfiles}
\begin{document}

\chapter{Collection of Sums}

\begin{equation*}
\sum_{k = 0}^{n} 1 = (n +1)
\end{equation*}

\noindent\makebox[\linewidth]{\rule{\paperwidth}{0.4pt}}

\begin{equation*}
	\sum_{k=0}^{n} k = \frac{n \cdot (n + 1)}{2}
\end{equation*}

\noindent\makebox[\linewidth]{\rule{\paperwidth}{0.4pt}}

\begin{equation*}
	\sum_{k=0}^{n} a + k = \frac{(n + 1) \cdot (2a + n)}{2}
\end{equation*}

\noindent\makebox[\linewidth]{\rule{\paperwidth}{0.4pt}}

\begin{equation*}
	\sum_{k = 1}^{n} 2k + 1 = n^2
\end{equation*}

\noindent\makebox[\linewidth]{\rule{\paperwidth}{0.4pt}}

\begin{equation*}
	\sum_{k = 0}^{n} 2k = n \cdot (n + 1)
\end{equation*}

\noindent\makebox[\linewidth]{\rule{\paperwidth}{0.4pt}}

\begin{equation*}
	\sum_{k = 0}^{n} k^2 = \frac{n \cdot (n + 1)^2}{6}
\end{equation*}

\noindent\makebox[\linewidth]{\rule{\paperwidth}{0.4pt}}

\begin{equation*}
	\sum_{k = 0}^{n} k^3 = \frac{n^2 \cdot (n + 1)^2}{4}
\end{equation*}

\noindent\makebox[\linewidth]{\rule{\paperwidth}{0.4pt}}

\begin{equation*}
	\sum_{k = 1}^{n} (2n - 1)^2 = \frac{n(4n^2 - 1)}{3}
\end{equation*}

\noindent\makebox[\linewidth]{\rule{\paperwidth}{0.4pt}}

\begin{equation*}
	\sum_{k = 1}^{n} (2n - 1)^3 = n^2(2n^2 - 1)
\end{equation*}

\noindent\makebox[\linewidth]{\rule{\paperwidth}{0.4pt}}

\begin{equation*}
	\sum_{k = 0}^{n} k^4 = \frac{n(n + 1)(2n + 1)(3n^2 + 3n - 1)}{30}
\end{equation*}

\noindent\makebox[\linewidth]{\rule{\paperwidth}{0.4pt}}

\begin{equation*}
	\sum_{k = 0}^{n} a^k = \frac{a^{n+1} - 1}{a -1}
\end{equation*}

\noindent\makebox[\linewidth]{\rule{\paperwidth}{0.4pt}}

\begin{equation*}
	\sum_{k = 0}^{n} a^{-k} = \frac{a^{-n}(a^{n+1} - 1)}{a - 1}
\end{equation*}

\noindent\makebox[\linewidth]{\rule{\paperwidth}{0.4pt}}

\newpage

\end{document}
