\documentclass[./\jobname.tex]{subfiles}
\begin{document}

\chapter{Collection of Trigonometric Identities}

\begin{equation*}
	sin(a) = \frac{1}{2i} \left( e^{ia} - e^{-ia} \right)
\end{equation*}

\begin{equation*}
	sin(a + b) = sin(a) \cdot cos(b) + cos(a) \cdot sin(b)
\end{equation*}

\begin{equation}
	sin(a - b) = sin(a) \cdot cos(b) - cos(a) \cdot sin(b)
\end{equation}

\begin{equation*}
	sin(2a) = 2 \cdot sin(a) \cdot cos(a)
\end{equation*}

\begin{equation*}
	sin(a)^2 = \frac{1}{2} \cdot (1 - cos(2a))
\end{equation*}

\begin{equation*}
	sin(a) + sin(b) = 2 \cdot sin\left( \frac{a + b}{2} \right) \cdot cos\left( \frac{a -b}{2} \right)
\end{equation*}

\begin{equation*}
	sin(a) - sin(b) = 2 \cdot cos\left( \frac{a + b}{2} \right) \cdot sin\left( \frac{a - b}{2} \right)
\end{equation*}

\noindent\makebox[\linewidth]{\rule{\paperwidth}{0.4pt}}

\begin{equation*}
	cos(a) = \frac{1}{2} \left( e^{ia} + e^{-ia} \right)
\end{equation*}

\begin{equation*}
	cos(a + b) = cos(a) \cdot cos(b) - sin(a) \cdot sin(b)
\end{equation*}

\begin{equation*}
	cos(a - b) = cos(a) \cdot cos(b) + sin(a) \cdot sin(b)
\end{equation*}

\begin{equation*}
	cos(2a) = cos(a)^2 - sin(a)^2
\end{equation*}

\begin{equation*}
	cos(a)^2 = \frac{1}{2} \cdot (1 + cos(2a))
\end{equation*}

\begin{equation*}
	cos(a)^2 = \frac{1}{1 + tan(a)^2}
\end{equation*}

\begin{equation*}
cos(a) + cos(b) = 2 \cdot cos\left( \frac{a + b}{2} \right) \cdot cos \left( \frac{a - b}{2} \right)
\end{equation*}

\begin{equation*}
cos(a) - cos(b) = -2 \cdot sin \left( \frac{a + b}{2} \right) \cdot sin \left( \frac{a - b}{2} \right)
\end{equation*}

\noindent\makebox[\linewidth]{\rule{\paperwidth}{0.4pt}}

\begin{equation*}
	sin(a)^2 + cos(a)^2 = 1
\end{equation*}

\begin{equation*}
	sin(a) \cdot cos(b) = \frac{1}{2} (sin(a + b) + sin(a-b))
\end{equation*}

\begin{equation*}
	cos(a) \cdot cos(b) = \frac{1}{2} (cos(a + b) + cos(a - b))
\end{equation*}

\begin{equation*}
	sin(a) \cdot sin(b) = \frac{1}{2} (cos(a-b) - cos(a+b))
\end{equation*}

\begin{equation*}
	arctan(a) + arctan\left( \frac{1}{a} \right) = \frac{\pi}{2}
\end{equation*}

\begin{equation*}
	e^{ia} = cos(a) + i \cdot sin(a)
\end{equation*}

\noindent\makebox[\linewidth]{\rule{\paperwidth}{0.4pt}}

\begin{equation*}
	sinh(a) = \frac{1}{2} = \left( e^a - e^{-a} \right)
\end{equation*}

\begin{equation*}
	cosh(a) = \frac{1}{2} = \left( e√¢ + e^{-a} \right)
\end{equation*}

\begin{equation*}
	tanh(a) = \frac{sinh(a)}{cosh(a)}
\end{equation*}

\begin{equation*}
	cosh(a)^2 - sinh(a)^2 = 1
\end{equation*}


\end{document}
